<?xml version="1.0"?>
<rdf:RDF xmlns="http://www.semanticweb.org/a.ihsan/ontologies/2021/8/untitled-ontology-45/"
     xml:base="http://www.semanticweb.org/a.ihsan/ontologies/2021/8/untitled-ontology-45/"
     xmlns:owl="http://www.w3.org/2002/07/owl#"
     xmlns:rdf="http://www.w3.org/1999/02/22-rdf-syntax-ns#"
     xmlns:xml="http://www.w3.org/XML/1998/namespace"
     xmlns:xsd="http://www.w3.org/2001/XMLSchema#"
     xmlns:rdfs="http://www.w3.org/2000/01/rdf-schema#"
     xmlns:skos="http://www.w3.org/2004/02/skos/core#">
    <owl:Ontology rdf:about="https://gitlab.com/azihsan/dislocation-ontology/-/raw/master/mdmc-nep-top-level"/>
    


    <!-- 
    ///////////////////////////////////////////////////////////////////////////////////////
    //
    // Annotation properties
    //
    ///////////////////////////////////////////////////////////////////////////////////////
     -->

    


    <!-- http://www.w3.org/2004/02/skos/core#definition -->

    <owl:AnnotationProperty rdf:about="http://www.w3.org/2004/02/skos/core#definition"/>
    


    <!-- 
    ///////////////////////////////////////////////////////////////////////////////////////
    //
    // Classes
    //
    ///////////////////////////////////////////////////////////////////////////////////////
     -->

    


    <!-- https://gitlab.com/azihsan/dislocation-ontology/-/raw/master/mdmc-nep-top-level/AnalyzedData -->

    <owl:Class rdf:about="https://gitlab.com/azihsan/dislocation-ontology/-/raw/master/mdmc-nep-top-level/AnalyzedData">
        <rdfs:subClassOf rdf:resource="https://gitlab.com/azihsan/dislocation-ontology/-/raw/master/mdmc-nep-top-level/Dataset"/>
        <skos:definition xml:lang="en">Identifiable Research data which is a result of Raw Data processing and Data Analysis, obtained with the use of Data Analysis Software. It is typically a data file but it can be potentially a data stream, or other form of data relevant in a particular data management context. Analysed Data is stored in a Data Repository, which may be the same in which Raw Data is stored. Analysed Data can be a part of Dataset.</skos:definition>
    </owl:Class>
    


    <!-- https://gitlab.com/azihsan/dislocation-ontology/-/raw/master/mdmc-nep-top-level/CorrelativeCharacterization -->

    <owl:Class rdf:about="https://gitlab.com/azihsan/dislocation-ontology/-/raw/master/mdmc-nep-top-level/CorrelativeCharacterization">
        <skos:definition xml:lang="en">The identifiable action of describing one or more Samples (depending on the particular research context) and connecting the different types of information from co-referenced (in time or space) multi-dimensional data. This may include using multiple Measurement Techniques to obtain complementary insights for a region of interest, as well as putting into relation features and properties of different sample areas across multiple length scales or over time.</skos:definition>
    </owl:Class>
    


    <!-- https://gitlab.com/azihsan/dislocation-ontology/-/raw/master/mdmc-nep-top-level/DataAnalysis -->

    <owl:Class rdf:about="https://gitlab.com/azihsan/dislocation-ontology/-/raw/master/mdmc-nep-top-level/DataAnalysis">
        <skos:definition xml:lang="en">The identifiable action of processing and/or combine and/or correlate Raw Data or/and Analysed Data. The analysis may be performed using Data Analysis Software and may be combined in chains or workflows. The data analysis includes data processing, correlative characterization, and data interpretation.</skos:definition>
    </owl:Class>
    


    <!-- https://gitlab.com/azihsan/dislocation-ontology/-/raw/master/mdmc-nep-top-level/DataAnalysisSoftware -->

    <owl:Class rdf:about="https://gitlab.com/azihsan/dislocation-ontology/-/raw/master/mdmc-nep-top-level/DataAnalysisSoftware">
        <skos:definition xml:lang="en">Software used for Data analysis (possibly including data rendering/visualization/plotting) and yielding Analyzed Data as an output. If Software is used for simulation (computer experiment), is it considered an Instrument and should be described as such.</skos:definition>
    </owl:Class>
    


    <!-- https://gitlab.com/azihsan/dislocation-ontology/-/raw/master/mdmc-nep-top-level/DataCollaborationPlatform -->

    <owl:Class rdf:about="https://gitlab.com/azihsan/dislocation-ontology/-/raw/master/mdmc-nep-top-level/DataCollaborationPlatform">
        <skos:definition xml:lang="en">A centralized operational information system where data inflows combine and allow authorized users to gather data and to draw on information, knowledge and insights.</skos:definition>
    </owl:Class>
    


    <!-- https://gitlab.com/azihsan/dislocation-ontology/-/raw/master/mdmc-nep-top-level/DataInterpretation -->

    <owl:Class rdf:about="https://gitlab.com/azihsan/dislocation-ontology/-/raw/master/mdmc-nep-top-level/DataInterpretation">
        <skos:definition xml:lang="en">The process of assigning meaning to the collected information, after an analytical and/or experimental Study, and determining the conclusions, significance, and implications of research findings, possibly in comparison with a predefined reference.</skos:definition>
    </owl:Class>
    


    <!-- https://gitlab.com/azihsan/dislocation-ontology/-/raw/master/mdmc-nep-top-level/DataProcessing -->

    <owl:Class rdf:about="https://gitlab.com/azihsan/dislocation-ontology/-/raw/master/mdmc-nep-top-level/DataProcessing">
        <skos:definition xml:lang="en">Data treatment to convert raw data into useful information for correlative characterization and interpretation. This may include filtering, scaling, fusion or compression of existing data as well as visualization, transformation and statistical data reduction. Typical tools for time or space related data conversion are derived from mathematics and/or informatics.</skos:definition>
    </owl:Class>
    


    <!-- https://gitlab.com/azihsan/dislocation-ontology/-/raw/master/mdmc-nep-top-level/DataRepository -->

    <owl:Class rdf:about="https://gitlab.com/azihsan/dislocation-ontology/-/raw/master/mdmc-nep-top-level/DataRepository">
        <skos:definition xml:lang="en">An operational information system for managing and organizing digital resources, particularly suitable for registering Datasets which are not likely to be altered again. For example, a Data Repository may host the Dataset supporting a publication. The Data Repository contains Metadata about the Datasets, as well as given rules for data access. Data Repository may be associated with a certain Institution or a group of them, or a certain Instrument or a group of them, or may be run by a third-party. Data Repository may or may not be directly used by Research Users.</skos:definition>
    </owl:Class>
    


    <!-- https://gitlab.com/azihsan/dislocation-ontology/-/raw/master/mdmc-nep-top-level/Dataset -->

    <owl:Class rdf:about="https://gitlab.com/azihsan/dislocation-ontology/-/raw/master/mdmc-nep-top-level/Dataset">
        <skos:definition xml:lang="en">A collection of scientifically related (depending on the research context) Research Data which can be Raw Data (including a result of computer simulation), Analysed Data, or other datasets, described by their related Metadata. The components of a dataset remain individually identifiable within the dataset.</skos:definition>
    </owl:Class>
    


    <!-- https://gitlab.com/azihsan/dislocation-ontology/-/raw/master/mdmc-nep-top-level/Equipment -->

    <owl:Class rdf:about="https://gitlab.com/azihsan/dislocation-ontology/-/raw/master/mdmc-nep-top-level/Equipment">
        <skos:definition xml:lang="en">Any kind of tool or device used during the course of an Experiment</skos:definition>
    </owl:Class>
    


    <!-- https://gitlab.com/azihsan/dislocation-ontology/-/raw/master/mdmc-nep-top-level/Experiment -->

    <owl:Class rdf:about="https://gitlab.com/azihsan/dislocation-ontology/-/raw/master/mdmc-nep-top-level/Experiment">
        <rdfs:subClassOf rdf:resource="https://gitlab.com/azihsan/dislocation-ontology/-/raw/master/mdmc-nep-top-level/Study"/>
        <skos:definition xml:lang="en">Identifiable and reproducible activity with a clear start time and clear finish time conducted by Research User who uses one or more Instruments to investigate or produce Sample and collects Raw Data about it. Experiment consists of (or includes â€“ in case of Sample Preparation) one or a series of Measurements. Experiment can be a computer simulation (computational experiment), or a combination of it with physical Measurements.</skos:definition>
    </owl:Class>
    


    <!-- https://gitlab.com/azihsan/dislocation-ontology/-/raw/master/mdmc-nep-top-level/Institution -->

    <owl:Class rdf:about="https://gitlab.com/azihsan/dislocation-ontology/-/raw/master/mdmc-nep-top-level/Institution">
        <skos:definition xml:lang="en">The hierarchical entity which owns the Instrument. For computer simulations, Institution may include hardware or/and software platforms or/and services that allow to order and manage computational experiments (so that the software platform serves the purpose of managing software modules that can be considered virtual Instruments).</skos:definition>
    </owl:Class>
    


    <!-- https://gitlab.com/azihsan/dislocation-ontology/-/raw/master/mdmc-nep-top-level/Instrument -->

    <owl:Class rdf:about="https://gitlab.com/azihsan/dislocation-ontology/-/raw/master/mdmc-nep-top-level/Instrument">
        <rdfs:subClassOf rdf:resource="https://gitlab.com/azihsan/dislocation-ontology/-/raw/master/mdmc-nep-top-level/Equipment"/>
        <skos:definition xml:lang="en">Identifiable Equipment that allows performing a Measurement and generated Raw Data in the course of an Experiment. Instrument is located in a Laboratory hosted by an Institution and used by one or more Research Users.  Instrument can be a software for computer simulation (a software module or/and a particular configuration of it).</skos:definition>
    </owl:Class>
    


    <!-- https://gitlab.com/azihsan/dislocation-ontology/-/raw/master/mdmc-nep-top-level/Laboratory -->

    <owl:Class rdf:about="https://gitlab.com/azihsan/dislocation-ontology/-/raw/master/mdmc-nep-top-level/Laboratory">
        <skos:definition xml:lang="en">Place where the instrument is located and the experiment is performed (could be also virtual)</skos:definition>
    </owl:Class>
    


    <!-- https://gitlab.com/azihsan/dislocation-ontology/-/raw/master/mdmc-nep-top-level/Measurement -->

    <owl:Class rdf:about="https://gitlab.com/azihsan/dislocation-ontology/-/raw/master/mdmc-nep-top-level/Measurement">
        <rdfs:subClassOf rdf:resource="https://gitlab.com/azihsan/dislocation-ontology/-/raw/master/mdmc-nep-top-level/Experiment"/>
        <skos:definition xml:lang="en">The act of generating a single self-consistent unit of Raw data for a Sample or a set of Samples which may be supported by a sample carrier during the Experiment using a particular Instrument under constant or varying controlled conditions, depending on the particular research context. Measurement is specific to Instrument: a research on the same Sample using a different Instrument implies a separate Measurement. Measurement can be a computer simulation, e.g. a particular run of a program using a particular model, configuration, or input(s).</skos:definition>
    </owl:Class>
    


    <!-- https://gitlab.com/azihsan/dislocation-ontology/-/raw/master/mdmc-nep-top-level/MeasurementTechnique -->

    <owl:Class rdf:about="https://gitlab.com/azihsan/dislocation-ontology/-/raw/master/mdmc-nep-top-level/MeasurementTechnique">
        <skos:definition xml:lang="en">A technique or technology corresponding to the method used to acquire Raw Data with a specific Instrument.</skos:definition>
    </owl:Class>
    


    <!-- https://gitlab.com/azihsan/dislocation-ontology/-/raw/master/mdmc-nep-top-level/Metadata -->

    <owl:Class rdf:about="https://gitlab.com/azihsan/dislocation-ontology/-/raw/master/mdmc-nep-top-level/Metadata">
        <rdfs:subClassOf rdf:resource="https://gitlab.com/azihsan/dislocation-ontology/-/raw/master/mdmc-nep-top-level/Dataset"/>
        <skos:definition xml:lang="en">A set of descriptive, structural and contextual information describing the context, content and structure of Research Data and/or Datasets, and their management through time. It describes information pertaining to research Projects, including (but not limited to) Research Users, Studies, Laboratories, Instruments, Measurements, Samples, Experiments, and corresponding Data Analyses. Metadata may include descriptions of how data and files are named, physically structured, and stored.</skos:definition>
    </owl:Class>
    


    <!-- https://gitlab.com/azihsan/dislocation-ontology/-/raw/master/mdmc-nep-top-level/Project -->

    <owl:Class rdf:about="https://gitlab.com/azihsan/dislocation-ontology/-/raw/master/mdmc-nep-top-level/Project">
        <skos:definition xml:lang="en">An enterprise (potentially individual but typically collaborative) of one or more Research Users, planned to perform one or more Studies in one or more Laboratories using one or more Instruments for taking one or more Measurements of one or more Samples during one or more Experiments, and corresponding Data Analyses. Laboratory, Instrument, Measurement, Experiment, and Sample can refer to computer simulation environment.</skos:definition>
    </owl:Class>
    


    <!-- https://gitlab.com/azihsan/dislocation-ontology/-/raw/master/mdmc-nep-top-level/RawData -->

    <owl:Class rdf:about="https://gitlab.com/azihsan/dislocation-ontology/-/raw/master/mdmc-nep-top-level/RawData">
        <rdfs:subClassOf rdf:resource="https://gitlab.com/azihsan/dislocation-ontology/-/raw/master/mdmc-nep-top-level/Dataset"/>
        <skos:definition xml:lang="en">The primary output of a Measurement, generated using a particular Instrument and collected by a Research User, before any subsequent processing, during an Experiment. Raw data is typically in the form of a data file but it can be potentially a data stream, or other form of data relevant in a particular data management context. Raw Data can be a result of a computer experiment (simulation). Raw Data can be a part of a Dataset.</skos:definition>
    </owl:Class>
    


    <!-- https://gitlab.com/azihsan/dislocation-ontology/-/raw/master/mdmc-nep-top-level/ResearchData -->

    <owl:Class rdf:about="https://gitlab.com/azihsan/dislocation-ontology/-/raw/master/mdmc-nep-top-level/ResearchData">
        <rdfs:subClassOf rdf:resource="https://gitlab.com/azihsan/dislocation-ontology/-/raw/master/mdmc-nep-top-level/Dataset"/>
        <skos:definition xml:lang="en">Data examined and considered as a basis for reasoning, discussion, or calculation in a research context. Examples of Research data include statistics, results of experiments, measurements, observations resulting from fieldwork, survey results, recordings and images. Within this definition, Raw data and Analysed Data are particular types of Research Data.</skos:definition>
    </owl:Class>
    


    <!-- https://gitlab.com/azihsan/dislocation-ontology/-/raw/master/mdmc-nep-top-level/ResearchUser -->

    <owl:Class rdf:about="https://gitlab.com/azihsan/dislocation-ontology/-/raw/master/mdmc-nep-top-level/ResearchUser">
        <skos:definition xml:lang="en">A person, a group of them, or an Institution (organization) who, within a Project, conducts Experiment on one or more Laboratories using one or more Instruments in order to collect and analyze Research Data, or is interested in data collected or analyzed by other Research Users on the same or other Facilities. Research User may be assigned with a role, e.g. to designate the user as a Principal Investigator.</skos:definition>
    </owl:Class>
    


    <!-- https://gitlab.com/azihsan/dislocation-ontology/-/raw/master/mdmc-nep-top-level/Sample -->

    <owl:Class rdf:about="https://gitlab.com/azihsan/dislocation-ontology/-/raw/master/mdmc-nep-top-level/Sample">
        <skos:definition xml:lang="en">Identifiable piece of material with distinctive properties (structural, chemical, dimensional and others), composed by one or more Sample Components, exposed to Instrument during a Measurement within a defined period of time. Sample may stand for a model or configuration or data input (or any combination of these) in computer simulations.</skos:definition>
    </owl:Class>
    


    <!-- https://gitlab.com/azihsan/dislocation-ontology/-/raw/master/mdmc-nep-top-level/SampleCarrier -->

    <owl:Class rdf:about="https://gitlab.com/azihsan/dislocation-ontology/-/raw/master/mdmc-nep-top-level/SampleCarrier">
        <skos:definition xml:lang="en">A structure used for carrying one or more samples, helpful for referencing, height adjustment, handling. It can be naked wafer, glass slide, sample holder, or an individually designed metal frame</skos:definition>
    </owl:Class>
    


    <!-- https://gitlab.com/azihsan/dislocation-ontology/-/raw/master/mdmc-nep-top-level/SampleComponent -->

    <owl:Class rdf:about="https://gitlab.com/azihsan/dislocation-ontology/-/raw/master/mdmc-nep-top-level/SampleComponent">
        <skos:definition xml:lang="en">Identifiable piece of material with distinctive properties (structural, chemical, dimensional and others), which constitutes a Sample.
It may include substrate, layer, mask, evaporants, coating, and the molecule(s) itself.</skos:definition>
    </owl:Class>
    


    <!-- https://gitlab.com/azihsan/dislocation-ontology/-/raw/master/mdmc-nep-top-level/SampleComponentSynthesis -->

    <owl:Class rdf:about="https://gitlab.com/azihsan/dislocation-ontology/-/raw/master/mdmc-nep-top-level/SampleComponentSynthesis">
        <skos:definition xml:lang="en">Production of each single Sample Component in controlled conditions, performed by a commercial enterprise, a Research User or someone else</skos:definition>
    </owl:Class>
    


    <!-- https://gitlab.com/azihsan/dislocation-ontology/-/raw/master/mdmc-nep-top-level/SamplePreparation -->

    <owl:Class rdf:about="https://gitlab.com/azihsan/dislocation-ontology/-/raw/master/mdmc-nep-top-level/SamplePreparation">
        <skos:definition xml:lang="en">Preliminary actions (physical changes or chemical reactions) typically carried out by a Research User on (or between) one or more Sample Components to produce a Sample, in order to perform a Measurement.</skos:definition>
    </owl:Class>
    


    <!-- https://gitlab.com/azihsan/dislocation-ontology/-/raw/master/mdmc-nep-top-level/Study -->

    <owl:Class rdf:about="https://gitlab.com/azihsan/dislocation-ontology/-/raw/master/mdmc-nep-top-level/Study">
        <rdfs:subClassOf rdf:resource="https://gitlab.com/azihsan/dislocation-ontology/-/raw/master/mdmc-nep-top-level/Project"/>
        <skos:definition xml:lang="en">A set of one or more experiments performed by one or more Research Users in one or more Laboratories using one or more Instruments for taking one or more Measurements of one or more Samples and corresponding Data analyses, which are part of the same Project.</skos:definition>
    </owl:Class>
</rdf:RDF>



<!-- Generated by the OWL API (version 4.5.9.2019-02-01T07:24:44Z) https://github.com/owlcs/owlapi -->

