<?xml version="1.0"?>
<rdf:RDF xmlns="https://purls.helmholtz-metadaten.de/prima/experiment#"
     xml:base="https://purls.helmholtz-metadaten.de/prima/experiment"
     xmlns:dal="https://purls.helmholtz-metadaten.de/prima/dal#"
     xmlns:owl="http://www.w3.org/2002/07/owl#"
     xmlns:rdf="http://www.w3.org/1999/02/22-rdf-syntax-ns#"
     xmlns:xml="http://www.w3.org/XML/1998/namespace"
     xmlns:xsd="http://www.w3.org/2001/XMLSchema#"
     xmlns:core="https://purls.helmholtz-metadaten.de/prima/core#"
     xmlns:rdfs="http://www.w3.org/2000/01/rdf-schema#"
     xmlns:skos="http://www.w3.org/2004/02/skos/core#"
     xmlns:vann="http://purl.org/vocab/vann/"
     xmlns:prima="https://purls.helmholtz-metadaten.de/prima/"
     xmlns:terms="http://purl.org/dc/terms/">
    <owl:Ontology rdf:about="https://purls.helmholtz-metadaten.de/prima/experiment">
        <terms:contributor xml:lang="en">Elda Osmenaj</terms:contributor>
        <terms:contributor xml:lang="en">Mirco Panighel</terms:contributor>
        <terms:created xml:lang="en">2022-10-16</terms:created>
        <terms:creator xml:lang="en">Ahmad Zainul Ihsan</terms:creator>
        <terms:creator xml:lang="en">Mehrdad Jalali</terms:creator>
        <terms:creator xml:lang="en">Rossella Aversa</terms:creator>
        <terms:license rdf:resource="http://creativecommons.org/licenses/by/3.0/"/>
        <terms:title xml:lang="en">PRIMA Ontology - Experiment Module</terms:title>
        <vann:preferredNamespacePrefix xml:lang="en">PRIMA</vann:preferredNamespacePrefix>
        <rdfs:comment xml:lang="en">This is the experiment module of the Provenance Information for Materials Science (PRIMA) Ontology</rdfs:comment>
        <rdfs:seeAlso rdf:resource="https://github.com/Materials-Data-Science-and-Informatics/MDMC-NEP-top-level-ontology"/>
        <owl:versionInfo xml:lang="en">1.0</owl:versionInfo>
    </owl:Ontology>
    


    <!-- 
    ///////////////////////////////////////////////////////////////////////////////////////
    //
    // Annotation properties
    //
    ///////////////////////////////////////////////////////////////////////////////////////
     -->

    


    <!-- http://purl.org/dc/terms/contributor -->

    <owl:AnnotationProperty rdf:about="http://purl.org/dc/terms/contributor"/>
    


    <!-- http://purl.org/dc/terms/created -->

    <owl:AnnotationProperty rdf:about="http://purl.org/dc/terms/created"/>
    


    <!-- http://purl.org/dc/terms/creator -->

    <owl:AnnotationProperty rdf:about="http://purl.org/dc/terms/creator"/>
    


    <!-- http://purl.org/dc/terms/description -->

    <owl:AnnotationProperty rdf:about="http://purl.org/dc/terms/description"/>
    


    <!-- http://purl.org/dc/terms/license -->

    <owl:AnnotationProperty rdf:about="http://purl.org/dc/terms/license"/>
    


    <!-- http://purl.org/dc/terms/title -->

    <owl:AnnotationProperty rdf:about="http://purl.org/dc/terms/title"/>
    


    <!-- http://purl.org/vocab/vann/preferredNamespacePrefix -->

    <owl:AnnotationProperty rdf:about="http://purl.org/vocab/vann/preferredNamespacePrefix"/>
    


    <!-- http://www.w3.org/2004/02/skos/core#definition -->

    <owl:AnnotationProperty rdf:about="http://www.w3.org/2004/02/skos/core#definition"/>
    


    <!-- https://purls.helmholtz-metadaten.de/prima/core#MDMCNEPGlossaryDefinition -->

    <owl:AnnotationProperty rdf:about="https://purls.helmholtz-metadaten.de/prima/core#MDMCNEPGlossaryDefinition">
        <rdfs:subPropertyOf rdf:resource="http://www.w3.org/2004/02/skos/core#definition"/>
    </owl:AnnotationProperty>
    

    <!-- 
    ///////////////////////////////////////////////////////////////////////////////////////
    //
    // Object Properties
    //
    ///////////////////////////////////////////////////////////////////////////////////////
     -->

    


    <!-- http://www.w3.org/ns/prov#atLocation -->

    <owl:ObjectProperty rdf:about="http://www.w3.org/ns/prov#atLocation"/>
    


    <!-- http://www.w3.org/ns/prov#used -->

    <owl:ObjectProperty rdf:about="http://www.w3.org/ns/prov#used"/>
    


    <!-- http://www.w3.org/ns/prov#wasAssociatedWith -->

    <owl:ObjectProperty rdf:about="http://www.w3.org/ns/prov#wasAssociatedWith"/>
    


    <!-- http://www.w3.org/ns/prov#wasDerivedFrom -->

    <owl:ObjectProperty rdf:about="http://www.w3.org/ns/prov#wasDerivedFrom"/>
    


    <!-- http://www.w3.org/ns/prov#wasGeneratedBy -->

    <owl:ObjectProperty rdf:about="http://www.w3.org/ns/prov#wasGeneratedBy"/>
    


    <!-- http://www.w3.org/ns/prov#wasInfluencedBy -->

    <owl:ObjectProperty rdf:about="http://www.w3.org/ns/prov#wasInfluencedBy"/>
    


    <!-- https://purls.helmholtz-metadaten.de/prima/experiment#carries -->

    <owl:ObjectProperty rdf:about="https://purls.helmholtz-metadaten.de/prima/experiment#carries">
        <owl:inverseOf rdf:resource="https://purls.helmholtz-metadaten.de/prima/experiment#isCarriedBy"/>
        <rdfs:domain rdf:resource="https://purls.helmholtz-metadaten.de/prima/experiment#SampleCarrier"/>
        <rdfs:range rdf:resource="https://purls.helmholtz-metadaten.de/prima/experiment#Sample"/>
        <rdfs:comment xml:lang="en">carries represents the relationship between sample carrier to sample.</rdfs:comment>
        <rdfs:label xml:lang="en">carries</rdfs:label>
    </owl:ObjectProperty>
    


    <!-- https://purls.helmholtz-metadaten.de/prima/experiment#hasMeasurement -->

    <owl:ObjectProperty rdf:about="https://purls.helmholtz-metadaten.de/prima/experiment#hasMeasurement">
        <owl:inverseOf rdf:resource="https://purls.helmholtz-metadaten.de/prima/experiment#isMeasurementOf"/>
        <rdfs:domain rdf:resource="https://purls.helmholtz-metadaten.de/prima/core#Experiment"/>
        <rdfs:range rdf:resource="https://purls.helmholtz-metadaten.de/prima/experiment#Measurement"/>
        <rdfs:comment xml:lang="en">hasMeasurement represents the relationship between experiment to measurement.</rdfs:comment>
        <rdfs:label xml:lang="en">has measurement</rdfs:label>
    </owl:ObjectProperty>
    


    <!-- https://purls.helmholtz-metadaten.de/prima/experiment#hasMeasurementTechnique -->

    <owl:ObjectProperty rdf:about="https://purls.helmholtz-metadaten.de/prima/experiment#hasMeasurementTechnique">
        <rdfs:domain rdf:resource="https://purls.helmholtz-metadaten.de/prima/experiment#Measurement"/>
        <rdfs:range rdf:resource="https://purls.helmholtz-metadaten.de/prima/experiment#MeasurementTechnique"/>
        <rdfs:comment xml:lang="en">hasMeasurementTechnique represents the relationship between measurement to measurement technique.</rdfs:comment>
        <rdfs:label xml:lang="en">has measurement technique</rdfs:label>
    </owl:ObjectProperty>
    


    <!-- https://purls.helmholtz-metadaten.de/prima/experiment#hasSampleComponent -->

    <owl:ObjectProperty rdf:about="https://purls.helmholtz-metadaten.de/prima/experiment#hasSampleComponent">
        <owl:inverseOf rdf:resource="https://purls.helmholtz-metadaten.de/prima/experiment#isSampleComponentOf"/>
        <rdfs:domain rdf:resource="https://purls.helmholtz-metadaten.de/prima/experiment#Sample"/>
        <rdfs:range rdf:resource="https://purls.helmholtz-metadaten.de/prima/experiment#SampleComponent"/>
        <rdfs:comment xml:lang="en">hasSampleComponent represents the relationship between sample to sample component</rdfs:comment>
        <rdfs:label xml:lang="en">has sample component</rdfs:label>
    </owl:ObjectProperty>
    


    <!-- https://purls.helmholtz-metadaten.de/prima/experiment#hasSampleComponentFabrication -->

    <owl:ObjectProperty rdf:about="https://purls.helmholtz-metadaten.de/prima/experiment#hasSampleComponentFabrication">
        <rdfs:domain rdf:resource="https://purls.helmholtz-metadaten.de/prima/core#Experiment"/>
        <rdfs:range rdf:resource="https://purls.helmholtz-metadaten.de/prima/experiment#SampleComponentFabrication"/>
        <rdfs:comment xml:lang="en">hasSampleComponentFabrication represents the relationship between experiment to sample component fabrication activity.</rdfs:comment>
        <rdfs:label xml:lang="en">has sample component fabrication</rdfs:label>
    </owl:ObjectProperty>
    


    <!-- https://purls.helmholtz-metadaten.de/prima/experiment#hasSamplePreparation -->

    <owl:ObjectProperty rdf:about="https://purls.helmholtz-metadaten.de/prima/experiment#hasSamplePreparation">
        <rdfs:domain rdf:resource="https://purls.helmholtz-metadaten.de/prima/core#Experiment"/>
        <rdfs:range rdf:resource="https://purls.helmholtz-metadaten.de/prima/experiment#SamplePreparation"/>
        <rdfs:comment xml:lang="en">hasSamplePreparation represents the relationship between experiment to sample preparation activity.</rdfs:comment>
        <rdfs:label xml:lang="en">has sample preparation</rdfs:label>
    </owl:ObjectProperty>
    


    <!-- https://purls.helmholtz-metadaten.de/prima/experiment#holds -->

    <owl:ObjectProperty rdf:about="https://purls.helmholtz-metadaten.de/prima/experiment#holds">
        <owl:inverseOf rdf:resource="https://purls.helmholtz-metadaten.de/prima/experiment#isHeldBy"/>
        <rdfs:domain rdf:resource="https://purls.helmholtz-metadaten.de/prima/experiment#SampleCarrier"/>
        <rdfs:range rdf:resource="https://purls.helmholtz-metadaten.de/prima/experiment#SampleHolder"/>
        <rdfs:comment xml:lang="en">holds represents the relationship between sample carrier to sample holder.</rdfs:comment>
        <rdfs:label xml:lang="en">holds</rdfs:label>
    </owl:ObjectProperty>
    


    <!-- https://purls.helmholtz-metadaten.de/prima/experiment#hosts -->

    <owl:ObjectProperty rdf:about="https://purls.helmholtz-metadaten.de/prima/experiment#hosts">
        <rdfs:domain rdf:resource="https://purls.helmholtz-metadaten.de/prima/experiment#Institution"/>
        <rdfs:range rdf:resource="https://purls.helmholtz-metadaten.de/prima/experiment#Laboratory"/>
        <rdfs:comment xml:lang="en">hosts represents the relationship between institution to laboratory.</rdfs:comment>
        <rdfs:label xml:lang="en">hosts</rdfs:label>
    </owl:ObjectProperty>
    


    <!-- https://purls.helmholtz-metadaten.de/prima/experiment#isCarriedBy -->

    <owl:ObjectProperty rdf:about="https://purls.helmholtz-metadaten.de/prima/experiment#isCarriedBy">
        <rdfs:comment xml:lang="en">isCarriedBy is the inverse property of carries.</rdfs:comment>
        <rdfs:label xml:lang="en">is carried by</rdfs:label>
    </owl:ObjectProperty>
    


    <!-- https://purls.helmholtz-metadaten.de/prima/experiment#isHeldBy -->

    <owl:ObjectProperty rdf:about="https://purls.helmholtz-metadaten.de/prima/experiment#isHeldBy">
        <rdfs:comment xml:lang="en">isHeldBy is the inverse property of holds.</rdfs:comment>
        <rdfs:label xml:lang="en">is held by</rdfs:label>
    </owl:ObjectProperty>
    


    <!-- https://purls.helmholtz-metadaten.de/prima/experiment#isMeasurementOf -->

    <owl:ObjectProperty rdf:about="https://purls.helmholtz-metadaten.de/prima/experiment#isMeasurementOf">
        <rdfs:comment xml:lang="en">isMeasurementOf is the inverse property of hasMeasurement.</rdfs:comment>
        <rdfs:label xml:lang="en">is measurement of</rdfs:label>
    </owl:ObjectProperty>
    


    <!-- https://purls.helmholtz-metadaten.de/prima/experiment#isSampleComponentOf -->

    <owl:ObjectProperty rdf:about="https://purls.helmholtz-metadaten.de/prima/experiment#isSampleComponentOf">
        <rdfs:subPropertyOf rdf:resource="http://www.w3.org/2002/07/owl#topObjectProperty"/>
        <rdfs:comment xml:lang="en">isSampleComponentOf is the inverse property of hasSampleComponent.</rdfs:comment>
        <rdfs:label xml:lang="en">is sample component of</rdfs:label>
    </owl:ObjectProperty>
    


    <!-- https://purls.helmholtz-metadaten.de/prima/experiment#wasOperatedBy -->

    <owl:ObjectProperty rdf:about="https://purls.helmholtz-metadaten.de/prima/experiment#wasOperatedBy">
        <rdfs:subPropertyOf rdf:resource="http://www.w3.org/ns/prov#wasInfluencedBy"/>
        <rdfs:domain rdf:resource="https://purls.helmholtz-metadaten.de/prima/experiment#Instrument"/>
        <rdfs:range rdf:resource="https://purls.helmholtz-metadaten.de/prima/core#ResearchUser"/>
        <rdfs:comment xml:lang="en">wasOperatedBy represents the provenance information that connects the agent that was operated by another agent, e.g., instrument was operated by research user.</rdfs:comment>
        <rdfs:label xml:lang="en">was operated by</rdfs:label>
    </owl:ObjectProperty>
    


    <!-- 
    ///////////////////////////////////////////////////////////////////////////////////////
    //
    // Data properties
    //
    ///////////////////////////////////////////////////////////////////////////////////////
     -->

    


    <!-- http://www.w3.org/ns/prov#endedAtTime -->

    <owl:DatatypeProperty rdf:about="http://www.w3.org/ns/prov#endedAtTime"/>
    


    <!-- http://www.w3.org/ns/prov#startedAtTime -->

    <owl:DatatypeProperty rdf:about="http://www.w3.org/ns/prov#startedAtTime"/>
    


    <!-- 
    ///////////////////////////////////////////////////////////////////////////////////////
    //
    // Classes
    //
    ///////////////////////////////////////////////////////////////////////////////////////
     -->

    


    <!-- http://www.w3.org/ns/prov#Activity -->

    <owl:Class rdf:about="http://www.w3.org/ns/prov#Activity"/>
    


    <!-- http://www.w3.org/ns/prov#Agent -->

    <owl:Class rdf:about="http://www.w3.org/ns/prov#Agent"/>
    


    <!-- http://www.w3.org/ns/prov#Entity -->

    <owl:Class rdf:about="http://www.w3.org/ns/prov#Entity"/>
    


    <!-- http://www.w3.org/ns/prov#Location -->

    <owl:Class rdf:about="http://www.w3.org/ns/prov#Location"/>
    


    <!-- http://www.w3.org/ns/prov#Organization -->

    <owl:Class rdf:about="http://www.w3.org/ns/prov#Organization">
        <rdfs:subClassOf rdf:resource="http://www.w3.org/ns/prov#Agent"/>
    </owl:Class>
    


    <!-- https://purls.helmholtz-metadaten.de/prima/core#Experiment -->

    <owl:Class rdf:about="https://purls.helmholtz-metadaten.de/prima/core#Experiment">
        <rdfs:subClassOf rdf:resource="http://www.w3.org/ns/prov#Activity"/>
        <rdfs:subClassOf>
            <owl:Restriction>
                <owl:onProperty rdf:resource="http://www.w3.org/ns/prov#atLocation"/>
                <owl:someValuesFrom rdf:resource="https://purls.helmholtz-metadaten.de/prima/experiment#Laboratory"/>
            </owl:Restriction>
        </rdfs:subClassOf>
        <rdfs:subClassOf>
            <owl:Restriction>
                <owl:onProperty rdf:resource="http://www.w3.org/ns/prov#wasAssociatedWith"/>
                <owl:someValuesFrom rdf:resource="https://purls.helmholtz-metadaten.de/prima/core#ResearchUser"/>
            </owl:Restriction>
        </rdfs:subClassOf>
        <rdfs:subClassOf>
            <owl:Restriction>
                <owl:onProperty rdf:resource="https://purls.helmholtz-metadaten.de/prima/experiment#hasMeasurement"/>
                <owl:someValuesFrom rdf:resource="https://purls.helmholtz-metadaten.de/prima/experiment#Measurement"/>
            </owl:Restriction>
        </rdfs:subClassOf>
        <rdfs:subClassOf>
            <owl:Restriction>
                <owl:onProperty rdf:resource="https://purls.helmholtz-metadaten.de/prima/experiment#hasSampleComponentFabrication"/>
                <owl:someValuesFrom rdf:resource="https://purls.helmholtz-metadaten.de/prima/experiment#SampleComponentFabrication"/>
            </owl:Restriction>
        </rdfs:subClassOf>
        <rdfs:subClassOf>
            <owl:Restriction>
                <owl:onProperty rdf:resource="https://purls.helmholtz-metadaten.de/prima/experiment#hasSamplePreparation"/>
                <owl:someValuesFrom rdf:resource="https://purls.helmholtz-metadaten.de/prima/experiment#SamplePreparation"/>
            </owl:Restriction>
        </rdfs:subClassOf>
        <rdfs:comment>Experiment is an identifiable and reproducible activity with a clear start time and end time, which may include a set of one or more sample component syntheses, sample preparations and/or measurements, performed by one or more research users.</rdfs:comment>
        <core:MDMCNEPGlossaryDefinition xml:lang="en">Identifiable and reproducible activity with a clear start time and end time, which may include a set of one or more sample component syntheses, sample preparations and/or measurements, performed by one or more research users. An experiment may be a simulation (computational experiment) or a combination of computational and physical measurement.</core:MDMCNEPGlossaryDefinition>
    </owl:Class>
    


    <!-- https://purls.helmholtz-metadaten.de/prima/core#ResearchUser -->

    <owl:Class rdf:about="https://purls.helmholtz-metadaten.de/prima/core#ResearchUser">
        <rdfs:subClassOf rdf:resource="http://www.w3.org/ns/prov#Agent"/>
        <rdfs:comment xml:lang="en">Research user is an agent or person, usually member of a project, who conducts any part of the experiment(s), or performs any of the steps of the data analysis lifecycle during the course of one or more studies.</rdfs:comment>
        <core:MDMCNEPGlossaryDefinition xml:lang="en">Person, usually member of a project, who conducts any part of the experiment(s), or performs any of the steps of the data analysis lifecycle during the course of one or more studies, in order to collect and/or analyse research data, or is interested in reusing research data collected by a third party (e.g., reference data) with the final aim to extract insights that support the answer to some specific research question (i.e., conclusions). Research users may be assigned with a role (e.g., principal investigator, instrument scientist, project member).</core:MDMCNEPGlossaryDefinition>
    </owl:Class>
    


    <!-- https://purls.helmholtz-metadaten.de/prima/dal#Experiment -->

    <owl:Class rdf:about="https://purls.helmholtz-metadaten.de/prima/dal#Experiment">
        <rdfs:subClassOf rdf:resource="http://www.w3.org/ns/prov#Entity"/>
        <rdfs:subClassOf>
            <owl:Restriction>
                <owl:onProperty rdf:resource="http://www.w3.org/ns/prov#wasGeneratedBy"/>
                <owl:someValuesFrom rdf:resource="https://purls.helmholtz-metadaten.de/prima/experiment#Measurement"/>
            </owl:Restriction>
        </rdfs:subClassOf>
        <rdfs:comment xml:lang="en">Raw data is research data which is the primary output of a measurement, collected by one or more research users using an instrument, before any subsequent data processing.</rdfs:comment>
        <core:MDMCNEPGlossaryDefinition xml:lang="en">Research Data which is the primary output of a measurement, collected by one or more research users using an instrument, before any subsequent data processing. Raw data may be the output of a simulation run (computational measurement). Raw data is typically in the form of a data file, but it may potentially be a data stream or any other form of data which is relevant in a particular data management context. Raw data may be stored in a data collaboration platform and/or in a data repository. Raw data may be part of a dataset.</core:MDMCNEPGlossaryDefinition>
    </owl:Class>
    


    <!-- https://purls.helmholtz-metadaten.de/prima/experiment#Equipment -->

    <owl:Class rdf:about="https://purls.helmholtz-metadaten.de/prima/experiment#Equipment">
        <rdfs:subClassOf rdf:resource="http://www.w3.org/ns/prov#Agent"/>
        <rdfs:subClassOf>
            <owl:Restriction>
                <owl:onProperty rdf:resource="http://www.w3.org/ns/prov#atLocation"/>
                <owl:someValuesFrom rdf:resource="https://purls.helmholtz-metadaten.de/prima/experiment#Laboratory"/>
            </owl:Restriction>
        </rdfs:subClassOf>
        <rdfs:comment xml:lang="en">Equipment is any kind of item, device, machine or other tool (also virtual) used by one or more research users to perform one or more sample component syntheses, sample preparations and/or measurements.</rdfs:comment>
        <core:MDMCNEPGlossaryDefinition xml:lang="en">Any kind of item, device, machine or other tool (also virtual) used by one or more research users to perform one or more sample component syntheses, sample preparations and/or measurements. Usually, the equipment is located in a laboratory hosted by an institution. According to this definition, an instrument is a particular type of equipment.</core:MDMCNEPGlossaryDefinition>
    </owl:Class>
    


    <!-- https://purls.helmholtz-metadaten.de/prima/experiment#Institution -->

    <owl:Class rdf:about="https://purls.helmholtz-metadaten.de/prima/experiment#Institution">
        <rdfs:subClassOf rdf:resource="http://www.w3.org/ns/prov#Organization"/>
        <rdfs:subClassOf>
            <owl:Restriction>
                <owl:onProperty rdf:resource="https://purls.helmholtz-metadaten.de/prima/experiment#hosts"/>
                <owl:someValuesFrom rdf:resource="https://purls.helmholtz-metadaten.de/prima/experiment#Laboratory"/>
            </owl:Restriction>
        </rdfs:subClassOf>
        <rdfs:comment xml:lang="en">Hierarchical entity which hosts one or more laboratories, including the virtual ones.</rdfs:comment>
        <core:MDMCNEPGlossaryDefinition xml:lang="en">Hierarchical entity which hosts one or more laboratories, including the virtual ones.</core:MDMCNEPGlossaryDefinition>
    </owl:Class>
    


    <!-- https://purls.helmholtz-metadaten.de/prima/experiment#Instrument -->

    <owl:Class rdf:about="https://purls.helmholtz-metadaten.de/prima/experiment#Instrument">
        <rdfs:subClassOf rdf:resource="https://purls.helmholtz-metadaten.de/prima/experiment#Equipment"/>
        <rdfs:subClassOf>
            <owl:Restriction>
                <owl:onProperty rdf:resource="https://purls.helmholtz-metadaten.de/prima/experiment#wasOperatedBy"/>
                <owl:someValuesFrom rdf:resource="https://purls.helmholtz-metadaten.de/prima/core#ResearchUser"/>
            </owl:Restriction>
        </rdfs:subClassOf>
        <rdfs:comment xml:lang="en">Instrument is identifiable piece of equipment used by one or more research users to perform a measurement and to generate raw data.</rdfs:comment>
        <core:MDMCNEPGlossaryDefinition xml:lang="en">Identifiable piece of equipment used by one or more research users to perform a measurement and to generate raw data. Instrument is located in a laboratory hosted by an institution. Instrument may also stand for a software, a software module and/or a particular configuration of it, used to perform a simulation run (computational measurement).</core:MDMCNEPGlossaryDefinition>
    </owl:Class>
    


    <!-- https://purls.helmholtz-metadaten.de/prima/experiment#Laboratory -->

    <owl:Class rdf:about="https://purls.helmholtz-metadaten.de/prima/experiment#Laboratory">
        <rdfs:subClassOf rdf:resource="http://www.w3.org/ns/prov#Location"/>
        <rdfs:comment xml:lang="en">Laboratory is place (could also be virtual) hosted by an institution, where one or more Instruments, as well as the equipment, are located and the measurement is performed.</rdfs:comment>
        <core:MDMCNEPGlossaryDefinition xml:lang="en">Place (could also be virtual) hosted by an Institution, where one or more Instruments, as well as the equipment, are located and the measurement is performed. Laboratory may be the hardware and/or the software platform and/or the services which allow to order and manage computational experiments. In this case, the software platform (virtual Laboratory) serves the purpose of managing software modules (virtual Instruments).</core:MDMCNEPGlossaryDefinition>
    </owl:Class>
    


    <!-- https://purls.helmholtz-metadaten.de/prima/experiment#Measurement -->

    <owl:Class rdf:about="https://purls.helmholtz-metadaten.de/prima/experiment#Measurement">
        <rdfs:subClassOf rdf:resource="http://www.w3.org/ns/prov#Activity"/>
        <rdfs:subClassOf>
            <owl:Restriction>
                <owl:onProperty rdf:resource="http://www.w3.org/ns/prov#used"/>
                <owl:someValuesFrom rdf:resource="https://purls.helmholtz-metadaten.de/prima/experiment#Sample"/>
            </owl:Restriction>
        </rdfs:subClassOf>
        <rdfs:subClassOf>
            <owl:Restriction>
                <owl:onProperty rdf:resource="https://purls.helmholtz-metadaten.de/prima/experiment#hasMeasurementTechnique"/>
                <owl:someValuesFrom rdf:resource="https://purls.helmholtz-metadaten.de/prima/experiment#MeasurementTechnique"/>
            </owl:Restriction>
        </rdfs:subClassOf>
        <rdfs:subClassOf>
            <owl:Restriction>
                <owl:onProperty rdf:resource="https://purls.helmholtz-metadaten.de/prima/experiment#isMeasurementOf"/>
                <owl:someValuesFrom rdf:resource="https://purls.helmholtz-metadaten.de/prima/core#Experiment"/>
            </owl:Restriction>
        </rdfs:subClassOf>
        <rdfs:subClassOf>
            <owl:Restriction>
                <owl:onProperty rdf:resource="http://www.w3.org/ns/prov#wasAssociatedWith"/>
                <owl:qualifiedCardinality rdf:datatype="http://www.w3.org/2001/XMLSchema#nonNegativeInteger">1</owl:qualifiedCardinality>
                <owl:onClass rdf:resource="https://purls.helmholtz-metadaten.de/prima/experiment#Instrument"/>
            </owl:Restriction>
        </rdfs:subClassOf>
        <rdfs:comment xml:lang="en">Measurement is identifiable and reproducible activity, performed by one or more research users, who generate a single self-consistent unit of raw data about a sample or a set of them using an instrument under constant or varying controlled conditions, depending on the particular research context.</rdfs:comment>
        <core:MDMCNEPGlossaryDefinition xml:lang="en">Identifiable and reproducible activity, performed by one or more research users, who generate a single self-consistent unit of raw data about a sample or a set of them using an instrument under constant or varying controlled conditions, depending on the particular research context. Measurement is specific to instrument: an investigation on the same sample conducted using a different instrument implies a different measurement. A measurement may also be performed during the sample component synthesis and/or the sample preparation, e.g., to characterize the resulting sample or sample component(s). A computational measurement may be a part of a simulation (computational experiment), e.g., a simulation run using a particular model, configuration or input(s).</core:MDMCNEPGlossaryDefinition>
    </owl:Class>
    


    <!-- https://purls.helmholtz-metadaten.de/prima/experiment#MeasurementTechnique -->

    <owl:Class rdf:about="https://purls.helmholtz-metadaten.de/prima/experiment#MeasurementTechnique">
        <rdfs:subClassOf rdf:resource="http://www.w3.org/ns/prov#Entity"/>
        <rdfs:comment xml:lang="en">Measurement technique is techique or technology corresponding to the method used during a measurement to collect raw data about a sample or a set of them with an instrument.</rdfs:comment>
        <core:MDMCNEPGlossaryDefinition xml:lang="en">Measurement technique is techique or technology corresponding to the method used during a measurement to collect raw data about a sample or a set of them with an instrument.</core:MDMCNEPGlossaryDefinition>
    </owl:Class>
    


    <!-- https://purls.helmholtz-metadaten.de/prima/experiment#Sample -->

    <owl:Class rdf:about="https://purls.helmholtz-metadaten.de/prima/experiment#Sample">
        <rdfs:subClassOf rdf:resource="http://www.w3.org/ns/prov#Entity"/>
        <rdfs:subClassOf>
            <owl:Restriction>
                <owl:onProperty rdf:resource="http://www.w3.org/ns/prov#wasDerivedFrom"/>
                <owl:someValuesFrom rdf:resource="https://purls.helmholtz-metadaten.de/prima/experiment#Sample"/>
            </owl:Restriction>
        </rdfs:subClassOf>
        <rdfs:subClassOf>
            <owl:Restriction>
                <owl:onProperty rdf:resource="http://www.w3.org/ns/prov#wasGeneratedBy"/>
                <owl:someValuesFrom rdf:resource="https://purls.helmholtz-metadaten.de/prima/experiment#SamplePreparation"/>
            </owl:Restriction>
        </rdfs:subClassOf>
        <rdfs:subClassOf>
            <owl:Restriction>
                <owl:onProperty rdf:resource="https://purls.helmholtz-metadaten.de/prima/experiment#hasSampleComponent"/>
                <owl:someValuesFrom rdf:resource="https://purls.helmholtz-metadaten.de/prima/experiment#SampleComponent"/>
            </owl:Restriction>
        </rdfs:subClassOf>
        <rdfs:subClassOf>
            <owl:Restriction>
                <owl:onProperty rdf:resource="https://purls.helmholtz-metadaten.de/prima/experiment#isCarriedBy"/>
                <owl:someValuesFrom rdf:resource="https://purls.helmholtz-metadaten.de/prima/experiment#SampleCarrier"/>
            </owl:Restriction>
        </rdfs:subClassOf>
        <rdfs:comment xml:lang="en">Sample is identifiable entity (typically a piece of material) with distinctive properties (structural, chemical, dimensional, functional and others), composed by one or more sample components, exposed to the Instrument during a measurement.</rdfs:comment>
        <core:MDMCNEPGlossaryDefinition xml:lang="en">Identifiable entity (typically a piece of material) with distinctive properties (structural, chemical, dimensional, functional and others), composed by one or more sample components, exposed to the Instrument during a measurement. Sample may be held by a sample holder and/or carried by a sample carrier during the measurement. Sample may also stand for a model, configuration or input (or any combination of them) of a simulation run (computational measurement).</core:MDMCNEPGlossaryDefinition>
    </owl:Class>
    


    <!-- https://purls.helmholtz-metadaten.de/prima/experiment#SampleCarrier -->

    <owl:Class rdf:about="https://purls.helmholtz-metadaten.de/prima/experiment#SampleCarrier">
        <rdfs:subClassOf rdf:resource="https://purls.helmholtz-metadaten.de/prima/experiment#Equipment"/>
        <rdfs:subClassOf>
            <owl:Restriction>
                <owl:onProperty rdf:resource="https://purls.helmholtz-metadaten.de/prima/experiment#carries"/>
                <owl:someValuesFrom rdf:resource="https://purls.helmholtz-metadaten.de/prima/experiment#Sample"/>
            </owl:Restriction>
        </rdfs:subClassOf>
        <rdfs:subClassOf>
            <owl:Restriction>
                <owl:onProperty rdf:resource="https://purls.helmholtz-metadaten.de/prima/experiment#holds"/>
                <owl:someValuesFrom rdf:resource="https://purls.helmholtz-metadaten.de/prima/experiment#SampleHolder"/>
            </owl:Restriction>
        </rdfs:subClassOf>
        <rdfs:comment xml:lang="en">Sample carrier is a piece of equipment used for carrying one or more samples and/or one or more sample holders, helpful, e.g., for referencing, handling or height adjustment.</rdfs:comment>
        <core:MDMCNEPGlossaryDefinition xml:lang="en">A piece of equipment used for carrying one or more samples and/or one or more sample holders, helpful, e.g., for referencing, handling or height adjustment. Sample carrier may be, e.g., a naked wafer, a glass slide or an individually designed metal frame.</core:MDMCNEPGlossaryDefinition>
    </owl:Class>
    


    <!-- https://purls.helmholtz-metadaten.de/prima/experiment#SampleComponent -->

    <owl:Class rdf:about="https://purls.helmholtz-metadaten.de/prima/experiment#SampleComponent">
        <rdfs:subClassOf rdf:resource="http://www.w3.org/ns/prov#Entity"/>
        <rdfs:subClassOf>
            <owl:Restriction>
                <owl:onProperty rdf:resource="http://www.w3.org/ns/prov#wasGeneratedBy"/>
                <owl:someValuesFrom rdf:resource="https://purls.helmholtz-metadaten.de/prima/experiment#SampleComponentFabrication"/>
            </owl:Restriction>
        </rdfs:subClassOf>
        <rdfs:subClassOf>
            <owl:Restriction>
                <owl:onProperty rdf:resource="https://purls.helmholtz-metadaten.de/prima/experiment#isSampleComponentOf"/>
                <owl:someValuesFrom rdf:resource="https://purls.helmholtz-metadaten.de/prima/experiment#Sample"/>
            </owl:Restriction>
        </rdfs:subClassOf>
        <rdfs:comment xml:lang="en">Sample component is identifiable entity (typically a piece of material) with distinctive properties (structural, chemical, dimensional, functional and others), which is fabricated during the sample component fabrication and is used during the sample preparation to produce a sample.</rdfs:comment>
        <core:MDMCNEPGlossaryDefinition xml:lang="en">Identifiable entity (typically a piece of material) with distinctive properties (structural, chemical, dimensional, functional and others), which is fabricated during the sample component fabrication and is used during the sample preparation to produce a sample. It may include substrate, layer, mask, evaporation material, coating, and the molecule itself.</core:MDMCNEPGlossaryDefinition>
    </owl:Class>
    


    <!-- https://purls.helmholtz-metadaten.de/prima/experiment#SampleComponentFabrication -->

    <owl:Class rdf:about="https://purls.helmholtz-metadaten.de/prima/experiment#SampleComponentFabrication">
        <rdfs:subClassOf rdf:resource="http://www.w3.org/ns/prov#Activity"/>
        <rdfs:subClassOf>
            <owl:Restriction>
                <owl:onProperty rdf:resource="http://www.w3.org/ns/prov#atLocation"/>
                <owl:someValuesFrom rdf:resource="https://purls.helmholtz-metadaten.de/prima/experiment#Laboratory"/>
            </owl:Restriction>
        </rdfs:subClassOf>
        <rdfs:subClassOf>
            <owl:Restriction>
                <owl:onProperty rdf:resource="http://www.w3.org/ns/prov#used"/>
                <owl:someValuesFrom rdf:resource="https://purls.helmholtz-metadaten.de/prima/experiment#SampleComponent"/>
            </owl:Restriction>
        </rdfs:subClassOf>
        <rdfs:subClassOf>
            <owl:Restriction>
                <owl:onProperty rdf:resource="http://www.w3.org/ns/prov#wasAssociatedWith"/>
                <owl:someValuesFrom rdf:resource="https://purls.helmholtz-metadaten.de/prima/core#ResearchUser"/>
            </owl:Restriction>
        </rdfs:subClassOf>
        <rdfs:subClassOf>
            <owl:Restriction>
                <owl:onProperty rdf:resource="http://www.w3.org/ns/prov#wasAssociatedWith"/>
                <owl:someValuesFrom rdf:resource="https://purls.helmholtz-metadaten.de/prima/experiment#Equipment"/>
            </owl:Restriction>
        </rdfs:subClassOf>
        <rdfs:subClassOf>
            <owl:Restriction>
                <owl:onProperty rdf:resource="http://www.w3.org/ns/prov#wasAssociatedWith"/>
                <owl:someValuesFrom rdf:resource="https://purls.helmholtz-metadaten.de/prima/experiment#Instrument"/>
            </owl:Restriction>
        </rdfs:subClassOf>
        <rdfs:subClassOf>
            <owl:Restriction>
                <owl:onProperty rdf:resource="https://purls.helmholtz-metadaten.de/prima/experiment#hasMeasurement"/>
                <owl:someValuesFrom rdf:resource="https://purls.helmholtz-metadaten.de/prima/experiment#Measurement"/>
            </owl:Restriction>
        </rdfs:subClassOf>
        <rdfs:comment xml:lang="en">Sample component fabrication is fabrication activity of a sample component in controlled conditions, performed by a commercial enterprise, a research user or a third party.</rdfs:comment>
        <core:MDMCNEPGlossaryDefinition xml:lang="en">Fabrication of a sample component in controlled conditions, performed by a commercial enterprise, a research user or a third party. Sample component fabrication may require the use of equipment and instrument(s). A measurement may also be performed during the sample component synthesis, e.g., to characterize the resulting sample component.</core:MDMCNEPGlossaryDefinition>
    </owl:Class>
    


    <!-- https://purls.helmholtz-metadaten.de/prima/experiment#SampleHolder -->

    <owl:Class rdf:about="https://purls.helmholtz-metadaten.de/prima/experiment#SampleHolder">
        <rdfs:subClassOf rdf:resource="https://purls.helmholtz-metadaten.de/prima/experiment#Equipment"/>
        <rdfs:subClassOf>
            <owl:Restriction>
                <owl:onProperty rdf:resource="https://purls.helmholtz-metadaten.de/prima/experiment#isHeldBy"/>
                <owl:someValuesFrom rdf:resource="https://purls.helmholtz-metadaten.de/prima/experiment#SampleCarrier"/>
            </owl:Restriction>
        </rdfs:subClassOf>
        <core:MDMCNEPGlossaryDefinition xml:lang="en">A piece of equipment that makes one or more samples accessible for a measurement, or holds them in place in the predefined position to be mounted inside the instrument (e.g., glass slide, TEM grid, tilting support). Sample holder(s) may be carried by a sample carrier.</core:MDMCNEPGlossaryDefinition>
    </owl:Class>
    


    <!-- https://purls.helmholtz-metadaten.de/prima/experiment#SamplePreparation -->

    <owl:Class rdf:about="https://purls.helmholtz-metadaten.de/prima/experiment#SamplePreparation">
        <rdfs:subClassOf rdf:resource="http://www.w3.org/ns/prov#Activity"/>
        <rdfs:subClassOf>
            <owl:Restriction>
                <owl:onProperty rdf:resource="http://www.w3.org/ns/prov#atLocation"/>
                <owl:someValuesFrom rdf:resource="https://purls.helmholtz-metadaten.de/prima/experiment#Laboratory"/>
            </owl:Restriction>
        </rdfs:subClassOf>
        <rdfs:subClassOf>
            <owl:Restriction>
                <owl:onProperty rdf:resource="http://www.w3.org/ns/prov#used"/>
                <owl:someValuesFrom rdf:resource="https://purls.helmholtz-metadaten.de/prima/experiment#Sample"/>
            </owl:Restriction>
        </rdfs:subClassOf>
        <rdfs:subClassOf>
            <owl:Restriction>
                <owl:onProperty rdf:resource="http://www.w3.org/ns/prov#used"/>
                <owl:someValuesFrom rdf:resource="https://purls.helmholtz-metadaten.de/prima/experiment#SampleComponent"/>
            </owl:Restriction>
        </rdfs:subClassOf>
        <rdfs:subClassOf>
            <owl:Restriction>
                <owl:onProperty rdf:resource="http://www.w3.org/ns/prov#wasAssociatedWith"/>
                <owl:someValuesFrom rdf:resource="https://purls.helmholtz-metadaten.de/prima/core#ResearchUser"/>
            </owl:Restriction>
        </rdfs:subClassOf>
        <rdfs:subClassOf>
            <owl:Restriction>
                <owl:onProperty rdf:resource="http://www.w3.org/ns/prov#wasAssociatedWith"/>
                <owl:someValuesFrom rdf:resource="https://purls.helmholtz-metadaten.de/prima/experiment#Equipment"/>
            </owl:Restriction>
        </rdfs:subClassOf>
        <rdfs:subClassOf>
            <owl:Restriction>
                <owl:onProperty rdf:resource="http://www.w3.org/ns/prov#wasAssociatedWith"/>
                <owl:someValuesFrom rdf:resource="https://purls.helmholtz-metadaten.de/prima/experiment#Instrument"/>
            </owl:Restriction>
        </rdfs:subClassOf>
        <rdfs:subClassOf>
            <owl:Restriction>
                <owl:onProperty rdf:resource="https://purls.helmholtz-metadaten.de/prima/experiment#hasMeasurement"/>
                <owl:someValuesFrom rdf:resource="https://purls.helmholtz-metadaten.de/prima/experiment#Measurement"/>
            </owl:Restriction>
        </rdfs:subClassOf>
        <rdfs:comment xml:lang="en">Sample preparation is identifiable and reproducible set of actions/activities (physical changes or chemical reactions) typically carried out by one or more research users to produce one or more samples and/or to make the sample(s) fit to perform a measurement.</rdfs:comment>
        <core:MDMCNEPGlossaryDefinition xml:lang="en">Identifiable and reproducible set of actions (physical changes or chemical reactions) typically carried out by one or more research users to produce one or more samples and/or to make the sample(s) fit to perform a measurement. The actions may be performed on (or between) one or more sample components, or on a sample. Sample preparation may require the use of equipment and Instrument(s). A Measurement may also be performed during the sample preparation, e.g., to characterize the resulting sample or sample component(s).</core:MDMCNEPGlossaryDefinition>
    </owl:Class>
</rdf:RDF>



<!-- Generated by the OWL API (version 4.5.9.2019-02-01T07:24:44Z) https://github.com/owlcs/owlapi -->

