@prefix : <https://purls.helmholtz-metadaten.de/prima/core#> .
@prefix dcterms: <http://purl.org/dc/terms/> .
@prefix owl: <http://www.w3.org/2002/07/owl#> .
@prefix prov: <http://www.w3.org/ns/prov#> .
@prefix rdf: <http://www.w3.org/1999/02/22-rdf-syntax-ns#> .
@prefix rdfs: <http://www.w3.org/2000/01/rdf-schema#> .
@prefix schema: <https://schema.org/> .
@prefix skos: <http://www.w3.org/2004/02/skos/core#> .
@prefix vann: <http://purl.org/vocab/vann/> .

dcterms:contributor a owl:AnnotationProperty .

dcterms:created a owl:AnnotationProperty .

dcterms:creator a owl:AnnotationProperty .

dcterms:description a owl:AnnotationProperty .

dcterms:license a owl:AnnotationProperty .

dcterms:title a owl:AnnotationProperty .

vann:preferredNamespacePrefix a owl:AnnotationProperty .

skos:closeMatch a owl:AnnotationProperty .

skos:exactMatch a owl:AnnotationProperty .

prov:endedAtTime a owl:DatatypeProperty .

prov:startedAtTime a owl:DatatypeProperty .

prov:used a owl:ObjectProperty .

<https://purls.helmholtz-metadaten.de/prima/core> a owl:Ontology ;
    dcterms:contributor "Elda Osmenaj"@en,
        "Mirco Panighel"@en ;
    dcterms:created "2024-01-26"@en ;
    dcterms:creator "Ahmad Zainul Ihsan"@en,
        "Mehrdad Jalali"@en,
        "Rossella Aversa"@en ;
    dcterms:license <http://creativecommons.org/licenses/by/3.0/> ;
    dcterms:title "PRIMA Ontology - Core Module"@en ;
    vann:preferredNamespacePrefix "PRIMA"@en ;
    rdfs:comment "This is the core module of the Provenance Information for Materials Science (PRIMA) Ontology"@en ;
    rdfs:seeAlso <https://github.com/Materials-Data-Science-and-Informatics/MDMC-NEP-top-level-ontology> ;
    owl:versionInfo "2.0"@en .

:ContactPerson a owl:Class ;
    rdfs:label "Contact Person"@en ;
    rdfs:comment "Person with knowledge of how to access, troubleshoot, or otherwise field issues related to the resource."@en ;
    rdfs:isDefinedBy <https://purls.helmholtz-metadaten.de/skosmos/prima/contactperson> ;
    rdfs:subClassOf :AgentRole ;
    skos:closeMatch <http://purl.org/datacite/v4.4/ContactPerson> ;
    skos:exactMatch <https://purls.helmholtz-metadaten.de/skosmos/prima/contactperson> .

:DataCollector a owl:Class ;
    rdfs:label "Data Collector"@en ;
    rdfs:comment "Person/institution responsible for finding or gathering/collecting data under the guidelines of the author(s) or Principal Investigator (PI)."@en ;
    rdfs:isDefinedBy <https://purls.helmholtz-metadaten.de/skosmos/prima/datacollector> ;
    rdfs:subClassOf :AgentRole ;
    skos:closeMatch <http://purl.org/datacite/v4.4/DataCollector> ;
    skos:exactMatch <https://purls.helmholtz-metadaten.de/skosmos/prima/datacollector> .

:Instrument a owl:Class ;
    rdfs:comment "Physical or virtual identifiable piece of Equipment used to perform a Data Acquisition and to generate Raw Data. The Instrument is located in a (physical or virtual) Laboratory hosted by an Institution and can be physically, virtually, and/or remotely accessed. A virtual Instrument may be any computational resource or HPC infrastructure (cloud infrastructure or supercomputer) needed to perform Calculations or Simulations."@en ;
    rdfs:isDefinedBy <https://purls.helmholtz-metadaten.de/skosmos/prima/instrument> ;
    rdfs:subClassOf :Equipment ;
    skos:exactMatch <https://purls.helmholtz-metadaten.de/skosmos/prima/instrument> .

:MDMCNEPGlossaryDefinition a owl:AnnotationProperty ;
    rdfs:subPropertyOf skos:definition .

:Material a owl:Class ;
    rdfs:comment "Broad term used to define a physical System, typically a substance or mixture of substances, in different states of matter or phases, of which something is composed or can be made. According to this definition, a Sample is constituted by at least one Material. Material(s) may undergo some kind of Processing and Treatment and/or Measurement."@en ;
    rdfs:isDefinedBy <https://purls.helmholtz-metadaten.de/skosmos/prima/material> ;
    rdfs:subClassOf :System ;
    skos:exactMatch <https://purls.helmholtz-metadaten.de/skosmos/prima/material> .

:ProjectLeader a owl:Class ;
    rdfs:label "Project Leader"@en ;
    rdfs:comment "Person officially designated as head of project team or sub- project team instrumental in the work necessary to development of the resource."@en ;
    rdfs:isDefinedBy <https://purls.helmholtz-metadaten.de/skosmos/prima/projectleader> ;
    rdfs:subClassOf :ProjectMember ;
    skos:closeMatch <http://purl.org/datacite/v4.4/ProjectLeader> ;
    skos:exactMatch <https://purls.helmholtz-metadaten.de/skosmos/prima/projectleader> .

:ProjectManager a owl:Class ;
    rdfs:label "Project Manager"@en ;
    rdfs:comment "Person officially designated as manager of a project. Project may consist of one or many project teams and sub-teams."@en ;
    rdfs:isDefinedBy <https://purls.helmholtz-metadaten.de/skosmos/prima/projectmanager> ;
    rdfs:subClassOf :ProjectMember ;
    skos:closeMatch <http://purl.org/datacite/v4.4/ProjectManager> ;
    skos:exactMatch <https://purls.helmholtz-metadaten.de/skosmos/prima/projectmanager> .

:RelatedPerson a owl:Class ;
    rdfs:label "Related Person"@en ;
    rdfs:comment "A person without a specifically defined role in the development of the resource, but who is someone the author wishes to recognize."@en ;
    rdfs:isDefinedBy <https://purls.helmholtz-metadaten.de/skosmos/prima/relatedperson> ;
    rdfs:subClassOf :AgentRole ;
    skos:closeMatch <http://purl.org/datacite/v4.4/RelatedPerson> ;
    skos:exactMatch <https://purls.helmholtz-metadaten.de/skosmos/prima/relatedperson> .

:Researcher a owl:Class ;
    rdfs:label "Researcher"@en ;
    rdfs:comment "A person involved in analysing data or the results of an experiment or formal study. May indicate an intern or assistant to one of the authors who helped with research but who was not so “key” as to be listed as an author."@en ;
    rdfs:isDefinedBy <https://purls.helmholtz-metadaten.de/skosmos/prima/researcher> ;
    rdfs:subClassOf :AgentRole ;
    skos:closeMatch <http://purl.org/datacite/v4.4/Researcher> ;
    skos:exactMatch <https://purls.helmholtz-metadaten.de/skosmos/prima/researcher> .

:Supervisor a owl:Class ;
    rdfs:label "Supervisor"@en ;
    rdfs:comment "Designated administrator over one or more groups/teams working to produce a resource, or over one or more steps of a development process."@en ;
    rdfs:isDefinedBy <https://purls.helmholtz-metadaten.de/skosmos/prima/supervisor> ;
    rdfs:subClassOf :AgentRole ;
    skos:closeMatch <http://purl.org/datacite/v4.4/Supervisor> ;
    skos:exactMatch <https://purls.helmholtz-metadaten.de/skosmos/prima/supervisor> .

:WorkPackageLeader a owl:Class ;
    rdfs:label "Work Package Leader"@en ;
    rdfs:comment "Person responsible for ensuring the comprehensive contents, versioning, and availability of the Work Package during the development of the resource."@en ;
    rdfs:isDefinedBy <https://purls.helmholtz-metadaten.de/skosmos/prima/workpackageleader> ;
    rdfs:subClassOf :AgentRole ;
    skos:closeMatch <http://purl.org/datacite/v4.4/WorkPackageLeader> ;
    skos:exactMatch <https://purls.helmholtz-metadaten.de/skosmos/prima/workpackageleader> .

:contributorType a owl:ObjectProperty ;
    rdfs:isDefinedBy "https://datacite-metadata-schema.readthedocs.io/en/4.5/appendices/appendix-1/contributorType/)" ;
    rdfs:subPropertyOf :performsAgentRole .

:hasStudy a owl:ObjectProperty ;
    rdfs:label "has study"@en ;
    rdfs:comment "hasStudy represents the relationship between project to study."@en ;
    rdfs:domain :Project ;
    rdfs:range :Study .

skos:definition a owl:AnnotationProperty .

prov:Activity a owl:Class .

:UserRole a owl:Class ;
    rdfs:label "User Role"@en ;
    rdfs:comment "The role of the Research User in a Project, in the context of a specific Study. Examples of User Role are: data curator, project leader, project member. User Role also determines the access rights which might be granted in the information system(s) used for data management (i.e., Data Collaboration Platform, Data Repository, Metadata Repository)."@en ;
    rdfs:isDefinedBy <https://purls.helmholtz-metadaten.de/skosmos/prima/userrole> ;
    skos:closeMatch <http://purl.org/datacite/v4.4/ContributorType> ;
    skos:exactMatch <https://purls.helmholtz-metadaten.de/skosmos/prima/userrole> .

:hasDataAcquisition a owl:ObjectProperty ;
    rdfs:label "has data acquisition"@en ;
    rdfs:comment "hasDataAcquisition represents the relationship between study to data acquisition"@en ;
    rdfs:range :DataAcquisition .

:hasDataAnalysis a owl:ObjectProperty ;
    rdfs:label "has data analysis"@en ;
    rdfs:comment "hasDataAnalysis represents the relationship between study to data analysis"@en ;
    rdfs:domain :Study ;
    rdfs:range :DataAnalysis .

:hasScientificPublication a owl:ObjectProperty ;
    rdfs:label "has scientific publication"@en ;
    rdfs:comment "hasScientificPublication represents the relationship between study to scientific publication"@en ;
    rdfs:domain :Study ;
    rdfs:range :ScientificPublication .

:isMemberOfProject a owl:ObjectProperty ;
    rdfs:label "is member of project"@en ;
    rdfs:comment "isMemberOfProject is the inverse of hasProjectMember, representing the relationship from research user to project"@en ;
    owl:inverseOf :hasProjectMember .

:operates a owl:ObjectProperty ;
    rdfs:label "operates"@en ;
    rdfs:comment "operates represents the relationship between equipment to research user"@en ;
    rdfs:domain :ResearchUser ;
    rdfs:range :Equipment .

:usesEquipment a owl:ObjectProperty ;
    rdfs:label "uses equipment"@en ;
    rdfs:comment "usesEquipment represents the relationship between data acquisition to equipment"@en ;
    rdfs:range :Equipment .

<https://purls.helmholtz-metadaten.de/prima/experiment#AcquisitionSoftware> a owl:Class ;
    rdfs:subClassOf prov:SoftwareAgent .

<https://w3id.org/pmd/co/DigitalEntity> a owl:Class ;
    rdfs:subClassOf prov:Entity .

<http://nfdi.fiz-karlsruhe.de/ontology/Specification> a owl:Class ;
    rdfs:subClassOf prov:Entity .

prov:SoftwareAgent a owl:Class ;
    rdfs:subClassOf prov:Agent .

prov:wasAssociatedWith a owl:ObjectProperty .

:Project a owl:Class ;
    rdfs:comment "Enterprise (potentially individual but typically collaborative) of one or more Research Users, planned to perform one or more Studies." ;
    rdfs:isDefinedBy <https://purls.helmholtz-metadaten.de/skosmos/prima/project> ;
    rdfs:subClassOf [ a owl:Restriction ;
            owl:onProperty :hasProjectMember ;
            owl:someValuesFrom :ResearchUser ],
        prov:Entity ;
    skos:exactMatch <https://purls.helmholtz-metadaten.de/skosmos/prima/project> .

:ProjectMember a owl:Class ;
    rdfs:label "Project Member"@en ;
    rdfs:comment "Person on the membership list of a designated project/project team."@en ;
    rdfs:isDefinedBy <https://purls.helmholtz-metadaten.de/skosmos/prima/projectmember> ;
    rdfs:subClassOf :AgentRole ;
    skos:closeMatch <http://purl.org/datacite/v4.4/ProjectMember> ;
    skos:exactMatch <https://purls.helmholtz-metadaten.de/skosmos/prima/projectmember> .

:ScientificPublication a owl:Class ;
    rdfs:label "Scientific Publication"@en ;
    rdfs:comment "Any of the following contributions, peer-reviewed or not: article in a scientific journal (and related supporting information), monograph, book or book chapter, conference proceedings, “grey literature” (informally published material having not gone through a standard publishing process, e.g., reports and highlights). A Scientific Publication typically reports the results and the conclusions of a Study, may be supplemented by Publication Data, and may be assigned a Persistent Identifier. A Scientific Publication may be attributed to some or to all the Research Users who are members of the Project."@en ;
    rdfs:isDefinedBy <https://purls.helmholtz-metadaten.de/skosmos/prima/scientificpublication> ;
    rdfs:subClassOf [ a owl:Restriction ;
            owl:onProperty prov:wasAttributedTo ;
            owl:someValuesFrom :ResearchUser ],
        prov:Entity ;
    skos:closeMatch <http://nfdi.fiz-karlsruhe.de/ontology/Publication>,
        schema:PublicationEvent ;
    skos:exactMatch <https://purls.helmholtz-metadaten.de/skosmos/prima/scientificpublication> .

:System a owl:Class ;
    rdfs:comment "Physical or digital entity or set of entities with distinctive properties (structural, chemical, dimensional, functional, or others) which is the subject of one or more actions or investigations. According to this definition, Sample, Material, and Model are particular types of System."@en ;
    rdfs:isDefinedBy <https://purls.helmholtz-metadaten.de/skosmos/prima/system> ;
    rdfs:subClassOf prov:Entity ;
    skos:exactMatch <https://purls.helmholtz-metadaten.de/skosmos/prima/system> .

:hasProjectMember a owl:ObjectProperty ;
    rdfs:label "has project member"@en ;
    rdfs:comment "hasProjectMember represents the relationship between project and its member, which is research user."@en ;
    owl:inverseOf :isMemberOfProject .

:hasSetting a owl:ObjectProperty ;
    rdfs:label "has setting"@en ;
    rdfs:comment "hasSetting represents the relationship between equipment or research software or acquisition software to settings"@en ;
    rdfs:domain [ a owl:Class ;
            owl:unionOf ( :Equipment :ResearchSoftware <https://purls.helmholtz-metadaten.de/prima/experiment#AcquisitionSoftware> ) ] ;
    rdfs:range :Settings .

:hasTechnique a owl:ObjectProperty ;
    rdfs:label "has technique"@en ;
    rdfs:comment "hasTechnique represents the relationship between data acquisition or data analysis to technique"@en ;
    rdfs:domain [ a owl:Class ;
            owl:unionOf ( :DataAcquisition :DataAnalysis ) ] ;
    rdfs:range :Technique .

:performsAgentRole a owl:ObjectProperty ;
    rdfs:label "performs agent role"@en ;
    rdfs:comment "performsAgentRole relates prov:Agent with AgentRole"@en ;
    rdfs:domain prov:Agent ;
    rdfs:range :AgentRole .

:usesResearchSoftware a owl:ObjectProperty ;
    rdfs:label "uses research software"@en ;
    rdfs:comment "usesResearchSoftware represents the relationship between data acquisition, data analysis, data processing, or data curation to research software"@en ;
    rdfs:domain [ a owl:Class ;
            owl:unionOf ( :DataAcquisition :DataAnalysis <https://purls.helmholtz-metadaten.de/prima/dal#DataProcessing> <https://purls.helmholtz-metadaten.de/prima/dataset#DataCuration> ) ] ;
    rdfs:range :ResearchSoftware .

<https://w3id.org/pmd/co/output> a owl:ObjectProperty .

:Settings a owl:Class ;
    rdfs:comment "Any set of configuration parameters which determine the operational conditions of Equipment (including Instrument), configure Acquisition Software and/or Research Software, and/or describe a Model (e.g., by specifying the type of solver user)."@en ;
    rdfs:isDefinedBy <https://purls.helmholtz-metadaten.de/skosmos/prima/settings> ;
    rdfs:subClassOf <http://nfdi.fiz-karlsruhe.de/ontology/Specification> ;
    skos:exactMatch <https://purls.helmholtz-metadaten.de/skosmos/prima/settings> .

:Study a owl:Class ;
    rdfs:comment "Set of all the processes and activities performed by one or more Research Users, who are part of the same Project, with the purpose of verifying, falsifying, or establishing the validity of a hypothesis and supporting the answer to some scientific research question. The output of a Study is usually reported in one or more Scientific Publications and may be supplemented by Publication Data." ;
    rdfs:isDefinedBy <https://purls.helmholtz-metadaten.de/skosmos/prima/study> ;
    rdfs:subClassOf [ a owl:Restriction ;
            owl:onProperty prov:wasAttributedTo ;
            owl:someValuesFrom :ResearchUser ],
        [ a owl:Restriction ;
            owl:onProperty :hasScientificPublication ;
            owl:someValuesFrom :ScientificPublication ],
        [ a owl:Restriction ;
            owl:onProperty :hasDataAcquisition ;
            owl:someValuesFrom :DataAcquisition ],
        [ a owl:Restriction ;
            owl:onProperty prov:wasAttributedTo ;
            owl:someValuesFrom :Project ],
        [ a owl:Restriction ;
            owl:onProperty :hasDataAnalysis ;
            owl:someValuesFrom :DataAnalysis ],
        <https://w3id.org/pmd/co/Process> ;
    skos:exactMatch <https://purls.helmholtz-metadaten.de/skosmos/prima/study> .

:Technique a owl:Class ;
    rdfs:comment "Any experimental, theoretical, or computational method with a specific aim, including but not limited to: process and/or treat Samples, prepare Models, acquire and/or analyze Research Data, using some Equipment."@en ;
    rdfs:isDefinedBy <https://purls.helmholtz-metadaten.de/skosmos/prima/technique> ;
    rdfs:subClassOf <http://nfdi.fiz-karlsruhe.de/ontology/Specification> ;
    skos:exactMatch <https://purls.helmholtz-metadaten.de/skosmos/prima/technique> .

<https://w3id.org/pmd/co/Process> a owl:Class ;
    rdfs:subClassOf prov:Activity .

<https://w3id.org/pmd/co/input> a owl:ObjectProperty .

prov:Agent a owl:Class .

prov:wasAttributedTo a owl:ObjectProperty .

:DataAcquisition a owl:Class ;
    rdfs:comment "Set of actions carried out by one or more Research Users, performed on a System or a set of them to generate a single self-consistent unit of Raw Data using a Technique, an Instrument and possibly other Equipment under constant or varying conditions described by Settings, depending on the particular research context. Data Acquisition may be an experimental (Measurement) or a computational (Calculation, Simulation) process. Data Acquisition is specific to a Technique: an investigation on the same System conducted using a different Technique implies a different Data Acquisition. The output of Data Acquisition is Raw Data."@en ;
    rdfs:isDefinedBy <https://purls.helmholtz-metadaten.de/skosmos/prima/dataacquisition> ;
    rdfs:subClassOf [ a owl:Restriction ;
            owl:onProperty :usesResearchSoftware ;
            owl:someValuesFrom :ResearchSoftware ],
        [ a owl:Restriction ;
            owl:onProperty :usesEquipment ;
            owl:someValuesFrom :Equipment ],
        [ a owl:Restriction ;
            owl:onProperty <https://w3id.org/pmd/co/input> ;
            owl:someValuesFrom :System ],
        [ a owl:Restriction ;
            owl:onProperty <https://w3id.org/pmd/co/output> ;
            owl:someValuesFrom :ResearchData ],
        [ a owl:Restriction ;
            owl:onProperty prov:wasAssociatedWith ;
            owl:someValuesFrom :ResearchUser ],
        [ a owl:Restriction ;
            owl:onProperty <https://w3id.org/pmd/co/input> ;
            owl:someValuesFrom :ResearchData ],
        [ a owl:Restriction ;
            owl:onProperty :hasTechnique ;
            owl:someValuesFrom :Technique ],
        <https://w3id.org/pmd/co/Process> ;
    skos:exactMatch <https://purls.helmholtz-metadaten.de/skosmos/prima/dataacquisition> .

:DataAnalysis a owl:Class ;
    rdfs:comment "Set of actions performed by one or more Research Users, possibly using a Technique and Research Software, on Research Data, typically Processed Data, to extract insights that support the answer to some scientific research question. Data Analysis may include: linear combination fitting, least-squares curve fitting, data modelling, pattern extraction and/or segmentation, data visualization. The output of Data Analysis is Analyzed Data."@en ;
    rdfs:isDefinedBy <https://purls.helmholtz-metadaten.de/skosmos/prima/dataanalysis> ;
    rdfs:subClassOf [ a owl:Restriction ;
            owl:onProperty :hasTechnique ;
            owl:someValuesFrom :Technique ],
        [ a owl:Restriction ;
            owl:onProperty <https://w3id.org/pmd/co/output> ;
            owl:someValuesFrom :ResearchData ],
        [ a owl:Restriction ;
            owl:onProperty <https://w3id.org/pmd/co/input> ;
            owl:someValuesFrom :ResearchData ],
        [ a owl:Restriction ;
            owl:onProperty prov:wasAssociatedWith ;
            owl:someValuesFrom :ResearchUser ],
        [ a owl:Restriction ;
            owl:onProperty :usesResearchSoftware ;
            owl:someValuesFrom :ResearchSoftware ],
        <https://w3id.org/pmd/co/Process> ;
    skos:exactMatch <https://purls.helmholtz-metadaten.de/skosmos/prima/dataanalysis> .

:ResearchData a owl:Class ;
    rdfs:comment "Data collected, created, or examined by one or more Research Users to be analyzed or considered as a basis for reasoning, discussion or calculation in a research context, with the purpose of generating, verifying, and/or validating original scientific claims that support the answer to some specific research question. According to this definition, Raw Data, Processed Data, Analyzed Data and Reference Data are particular types of Research Data. Research Data is typically in the form of one or more data files, but it may potentially be a data stream or any other form of data which is relevant in a particular data management context. Research Data may be described by Metadata and may be stored in a Data Collaboration Platform and/or in a Data Repository. Research Data may undergo some kind of Data Curation and be aggregated into a Dataset."@en ;
    rdfs:isDefinedBy <https://purls.helmholtz-metadaten.de/skosmos/prima/researchdata> ;
    rdfs:subClassOf [ a owl:Restriction ;
            owl:onProperty prov:wasAttributedTo ;
            owl:someValuesFrom :ResearchUser ],
        <https://w3id.org/pmd/co/DigitalEntity> ;
    skos:exactMatch <https://purls.helmholtz-metadaten.de/skosmos/prima/researchdata> .

:ResearchSoftware a owl:Class ;
    rdfs:comment "Any software used to process, analyze, or visualize Research Data (including data rendering and or plotting)."@en ;
    rdfs:isDefinedBy <https://purls.helmholtz-metadaten.de/skosmos/prima/researchsoftware> ;
    rdfs:subClassOf [ a owl:Restriction ;
            owl:onProperty :hasSetting ;
            owl:someValuesFrom :Settings ],
        prov:SoftwareAgent ;
    skos:exactMatch <https://purls.helmholtz-metadaten.de/skosmos/prima/researchsoftware> .

prov:Entity a owl:Class .

:Equipment a owl:Class ;
    rdfs:comment "Any kind of physical or virtual item, device, machine or other tool located in a Laboratory hosted by an Institution, which can be physically, virtually, and/or remotely accessed to perform any of the processes during the course of a Study, by applying a Technique. Equipment is usually an investment. According to this definition, an Instrument is a particular type of Equipment."@en ;
    rdfs:isDefinedBy <https://purls.helmholtz-metadaten.de/skosmos/prima/equipment> ;
    rdfs:subClassOf [ a owl:Restriction ;
            owl:onProperty :hasSetting ;
            owl:someValuesFrom :Settings ],
        prov:Agent ;
    skos:exactMatch <https://purls.helmholtz-metadaten.de/skosmos/prima/equipment> .

:ResearchUser a owl:Class ;
    rdfs:comment "Person, usually member of a Project, who conducts any part of the Study to collect and/or to analyze Research Data, and/or reuses Reference Data to extract insights that support the answer to some specific research question, usually reported in one or more Scientific Publications. A Research User may be assigned with a User Role."@en ;
    rdfs:isDefinedBy <https://purls.helmholtz-metadaten.de/skosmos/prima/researchuser> ;
    rdfs:subClassOf [ a owl:Restriction ;
            owl:onProperty :performsAgentRole ;
            owl:someValuesFrom :AgentRole ],
        [ a owl:Restriction ;
            owl:onProperty :operates ;
            owl:someValuesFrom :Equipment ],
        prov:Agent ;
    skos:exactMatch <https://purls.helmholtz-metadaten.de/skosmos/prima/researchuser> .

:AgentRole a owl:Class ;
    rdfs:comment "A functional role that an Agent can perform within a research context. Roles define the responsibilities and capabilities of agents in conducting research activities."@en ;
    owl:equivalentClass :UserRole .

